ulib/mk_int.sh
@@ -10,3 +10,14 @@ let n = $i
 EOF
   cat FStar.IntN.fstp >> $f
 done
+
+for i in 8 16 31 32 63 64; do
+  f=FStar.UInt$i.fst
+  cat > $f <<EOF
+module FStar.UInt$i
+
+let n = $i
+
+EOF
+  cat FStar.IntN.fstp >> $f
+done
